NatTM: Finish iter and implement add with iter

TM/Code/NatTM.v
@@ -2,6 +2,8 @@ Require Import TM.Code.CodeTM TM.Code.MatchNat.
 Require Import TM.Basic.Mono Basic.Nop Combinators.Combinators.
 Require Import TM.LiftMN TM.LiftSigmaTau.
 Require Import TM.Compound.TMTac.
+Require Import TM.Code.Copy.
+Require Import Coq.Init.Nat.
 
 
 Definition is_zero (n : nat) :=
@@ -21,6 +23,73 @@ Lemma is_zero_correct (n : nat) :
 Proof. destruct n; cbn; split; congruence. Qed.
 
 
+(*
+ * This definition of [tail_plus] differs from the definition of [tail_plus] in the standard library,
+ * only that it is recursive over the second number.
+ *)
+
+Search tail_plus.
+
+Fixpoint tail_plus (m n : nat) { struct n } : nat :=
+  match n with
+  | O => m
+  | S n' => tail_plus (S m) n'
+  end.
+
+Lemma plus_tail_plus (m n : nat) :
+  m + n = tail_plus m n.
+Proof.
+  revert m. induction n as [ | n' IH ]; intros.
+  - cbn. omega.
+  - cbn.  rewrite <- IH. omega.
+Qed.
+
+
+Fixpoint tail_mult_acc (a m n : nat) {struct n} :=
+  match n with
+  | O => a
+  | S n' => tail_mult_acc (tail_plus a m) m n'
+  end.
+
+Definition tail_mult (m n : nat) := tail_mult_acc 0 m n.
+
+Lemma mult_tail_mult_aux (a m n : nat) :
+  a + m * n = tail_mult_acc a m n.
+Proof.
+  revert a m. induction n as [ | n' IH]; intros.
+  - cbn. omega.
+  - cbn. rewrite <- IH. rewrite <- plus_tail_plus. rewrite Nat.mul_succ_r. omega.
+Qed.
+
+Lemma mult_tail_mult (m n : nat) :
+  m * n = tail_mult m n.
+Proof. pose proof (mult_tail_mult_aux 0 m n) as L. cbn in L. auto. Qed.
+
+
+(* [tail_pow] is missing at all *)
+Print pow.
+Fixpoint tail_pow_acc (a m n : nat) {struct n} : nat :=
+  match n with
+  | O => a
+  | S n' => tail_pow_acc (tail_mult a m) m n'
+  end.
+
+Definition tail_pow (m n : nat) := tail_pow_acc 1 m n.
+
+Lemma pow_tail_pow_aux (a m n : nat) :
+  a * pow m n = tail_pow_acc a m n.
+Proof.
+  revert a m. induction n as [ | n' IH]; intros.
+  - cbn. omega.
+  - cbn. rewrite <- IH. rewrite <- mult_tail_mult. eapply Nat.mul_assoc.
+Qed.
+
+Lemma pow_tail_pow (m n : nat) :
+  pow m n = tail_pow m n.
+Proof. pose proof (pow_tail_pow_aux 1 m n) as L. cbn in L. unfold tail_pow. omega. Qed.
+
+
+
 Lemma MatchNat_Computes_Pred :
   MatchNat ⊨c(5) Computes_Rel_p (Fin.F1) (Fin.F1) _ _ pred is_not_zero.
 Proof.
@@ -36,32 +105,32 @@ Proof.
 Qed.
 
 
+(** * First-order [nat] iteration machines *)
 
-(* Tail recursive funktions over [nat] *)
-Section FoldNat.
+Section Iter1.
 
-  Variable Y : finType.
   Variable f : nat -> nat.
 
-  Fixpoint iter (x y : nat) {struct x} : nat :=
-    match x with
-    | 0 => y
-    | S x' => iter x' (f y)
+  (* [x] is the accu. We iterate over [y]. *)
+  Fixpoint iter (x y : nat) {struct y} : nat :=
+    match y with
+    | 0 => x
+    | S y' => iter (f x) y'
     end.
 
   Variable M1 : { M : mTM (bool^+) 1 & states M -> unit }.
   Hypothesis M1_computes : M1 ⊫ Computes_Rel Fin.F1 Fin.F1 _ _ f.
 
   Definition iter_step (x y : nat) : nat :=
-    match x with
-    | 0 => y
-    | S _ => f y
+    match y with
+    | 0 => x
+    | S _ => f x
     end.
 
 
   Definition Iter_step : { M : mTM _ 2 & states M -> bool * unit } :=
-    If (Inject MatchNat [|Fin.F1|])
-       (Inject M1 [|Fin.FS Fin.F1|];; Nop _ _ (true, tt))
+    If (Inject MatchNat [|Fin.FS Fin.F1|])
+       (Return (Inject M1 [|Fin.F1|]) (true, tt))
        (Nop _ _ (false, tt)).
   
 
@@ -73,8 +142,8 @@ Section FoldNat.
   Definition tailRec_step_param : nat -> bool * unit := fun n => (is_not_zero n, tt).
 
   Lemma Iter_step_Computes :
-    Iter_step ⊫ Computes_Rel_p (Fin.F1) (Fin.F1) _ _ pred tailRec_step_param ∩
-                   Computes2_Rel (Fin.F1) (Fin.FS Fin.F1) (Fin.FS Fin.F1) _ _ _ iter_step.
+    Iter_step ⊫ Computes_Rel_p (Fin.FS Fin.F1) (Fin.FS Fin.F1) _ _ pred tailRec_step_param ∩
+                   Computes2_Rel (Fin.F1) (Fin.FS Fin.F1) (Fin.F1) _ _ _ iter_step.
   Proof.
     eapply WRealise_monotone.
     {
@@ -83,29 +152,22 @@ Section FoldNat.
     }
     {
       intros tin (yout, tout). split.
-      - intros n HEn. destruct H; hnf in H.
-        + destruct H as (tmid&(H1&H2)&([]&t)&H3&->&->); hnf in H1, H2, H3. simpl_not_in.
-          specialize (H1 n). spec_assert H1 as (n'&->&H1). { unfold reorder. now simpl_vector. } cbn in *. split; auto.
-          destruct H3 as (H3&H4); hnf in H3, H4. simpl_not_in. rewrite <- H2, H4 in *; clear H2 H4. auto.
-        + destruct H as (tmid&(H1&H2)&->&->); hnf in H1, H2. simpl_not_in. specialize (H1 n).
-          spec_assert H1 as (->&H1). { unfold reorder. now simpl_vector. } cbn. auto.
-      - intros n m HEn Hem. destruct H; hnf in H.
-        + destruct H as (tmid&(H1&H2)&([]&t)&H3&->&->); hnf in H1, H2, H3. simpl_not_in.
-          specialize (H1 n). spec_assert H1 as (n'&->&H1). { unfold reorder. now simpl_vector. } cbn in *. auto.
-          destruct H3 as (H3&H4); hnf in H3, H4. simpl_not_in. rewrite <- H2, H4 in *; clear H2 H4. auto.
-        + destruct H as (tmid&(H1&H2)&->&->); hnf in H1, H2. simpl_not_in. specialize (H1 n). spec_assert H1 as (->&H1).
-          { unfold reorder. now simpl_vector. } cbn in *. rewrite H2 in *; clear H2. auto.
+      - intros n HEn. destruct H; TMSimp.
+        + specialize (H n HEn) as (n'&->&H). cbn. auto.
+        + specialize (H n HEn) as (->&H). cbn. auto.
+      - intros n m HEn HEm. destruct H; TMSimp.
+        + specialize (H m HEm) as (n'&->&H). cbn. auto.
+        + specialize (H m HEm) as (->&H). cbn. auto.
     }
   Qed.
 
-  
   Lemma iter_eta (x y : nat) :
-    iter (Init.Nat.pred x) (iter_step x y) = iter x y.
+    iter (iter_step x y) (Init.Nat.pred y) = iter x y.
   Proof. destruct x, y; cbn; omega. Qed.
 
 
   Lemma Iter_Computes :
-    Iter ⊫ Computes2_Rel (Fin.F1) (Fin.FS Fin.F1) (Fin.FS Fin.F1) _ _ _ iter.
+    Iter ⊫ Computes2_Rel (Fin.F1) (Fin.FS Fin.F1) (Fin.F1) _ _ _ iter.
   Proof.
     eapply WRealise_monotone.
     {
@@ -113,12 +175,16 @@ Section FoldNat.
     }
     {
       hnf. intros tin ((), tout) H. destruct H as (tmid&H1&H2&H3).
-      revert tout H2 H3. induction H1 as [ tin | tin tmid tout H1 H2 IH]; intros; hnf in *; intros.
-      - specialize (H2 _ H) as (H2&H2'). specialize (H3 _ _ H H0). cbn in *.
-        unfold tailRec_step_param in *. destruct x, y; cbn in *; inv H2'; auto.
-      - cbn in *. destruct H1 as (()&H11&H12).
-        hnf in H11, H12. specialize (H11 x H) as (H11&H11'). specialize (H12 x y H H4).
-        specialize (IH _ H0 H3). specialize (IH _ _ H11 H12). rewrite iter_eta in IH. auto.
+      induction H1 as [ tin | tin tmid1 tmid2 HStar _ IH]; intros; hnf in *; intros.
+      - specialize (H2 _ H0) as (H2&H2'). specialize (H3 _ _ H H0).
+        unfold tailRec_step_param in H2'. destruct y; cbn in H2'; try congruence.
+        cbn. auto.
+      - cbn in *. do 2 spec_assert IH; auto.
+        destruct HStar as (() & HStar1&HStar2).
+        specialize (HStar1 y H0) as (HStar1&HStar1').
+        specialize (HStar2 x y H H0).
+        specialize (IH _ _ HStar2 HStar1).
+        now rewrite iter_eta in IH.
     }
   Qed.
 
@@ -129,7 +195,12 @@ Section FoldNat.
   Hypothesis M1_terminates : projT1 M1 ↓ (fun tin k => exists y, tin[@Fin.F1] ≂ y /\ M1_runtime y <= k).
 
   Lemma Iter_step_terminates :
-    projT1 Iter_step ↓ (fun tin k => exists x y, tin[@Fin.F1] ≂ x /\ tin[@Fin.FS Fin.F1] ≂ y /\ 8 + M1_runtime y <= k).
+    projT1 Iter_step ↓
+           (fun tin k => exists x y, tin[@Fin.F1] ≂ x /\ tin[@Fin.FS Fin.F1] ≂ y /\
+                             match y with
+                             | O => 6
+                             | S y' => 6 + M1_runtime x
+                             end <= k).
   Proof.
     unfold Iter_step.
     eapply TerminatesIn_monotone.
@@ -140,144 +211,114 @@ Section FoldNat.
     }
     {
       intros tin i (x&y&HT1&HT2&HT3).
-      exists 5. exists (2 + M1_runtime y). repeat split.
-      - omega.
-      - hnf. omega.
-      - intros tout b (H1&H2).
-        hnf in H1. specialize (H1 x). cbn in H1. specialize (H1 ltac:(eauto)) as (H1&H1').
-        hnf in H2. simpl_not_in.
-        destruct b.
-        + exists (M1_runtime y), 0. repeat split.
-          * omega.
-          * hnf. eexists. split. cbn. rewrite <- H2. eauto. omega.
-          * intros. omega.
+      destruct y as [ | y' ].
+      - exists 5, 0. repeat split.
         + omega.
+        + cbn. omega.
+        + intros tout b (HComp1&HComp2). cbn in HComp1, HComp2. specialize (HComp1 O HT2) as (HComp11&HComp12).
+          cbn in HComp12. subst. omega.
+      - exists 5, (M1_runtime x). repeat split.
+        + omega.
+        + hnf. omega.
+        + intros tout b (H1&H2).
+          hnf in H1. cbn -[add] in *. simpl_not_in. rewrite H2 in *; clear H2. specialize (H1 (S y') HT2) as (H1&->).
+          cbn. exists x. split. assumption. auto.
     }
   Qed.
 
-  
 
-  (* TODO weiter verallgemeinierte Version implementieren... *)
-
-End FoldNat.
-
-
-
-
-Definition Add_step : { M : mTM _ 2 & states M -> bool * unit } :=
-  If (Inject MatchNat [|Fin.F1|])
-     (Inject Constr_S [|Fin.FS Fin.F1|];; Nop _ _ (true, tt))
-     (Nop _ _ (false, tt)).
-
-Definition add_step__f : nat -> nat -> nat :=
-  fun n m =>
+  Fixpoint Iter_steps (m n : nat) { struct n } : nat :=
     match n with
-    | 0 => m
-    | S _ => S m
+    | O => 6
+    | S n' => 7 + M1_runtime m + Iter_steps (f m) n'
     end.
 
-Definition add_step__p1 : nat -> bool * unit := fun n => (is_not_zero n, tt).
+  Lemma Iter_steps_ge5 (m n : nat) :
+    5 <= Iter_steps m n.
+  Proof. destruct n; cbn; omega. Qed.
 
-Definition add_step__p2 : nat -> nat -> bool * unit := fun n m => (is_not_zero n, tt).
 
-Lemma Add_step_Computes :
-  Add_step ⊨c(12)
-           Computes_Rel_p (Fin.F1) (Fin.F1) _ _ pred add_step__p1 ∩
-           Computes2_Rel_p (Fin.F1) (Fin.FS Fin.F1) (Fin.FS Fin.F1) _ _ _ add_step__f add_step__p2.
+  Lemma Iter_steps_homogene (m n k : nat) :
+    (forall x, M1_runtime x <= k) ->
+    Iter_steps m n <= 6 + (7 + k) * n.
+  Proof.
+    revert m. induction n as [ | n' IH]; intros; cbn -[add mult] in *.
+    - omega.
+    - specialize (IH (f m) H). pose proof (H (f m)) as H1. pose proof (H m) as H2.
+      rewrite !Nat.mul_succ_r.
+      rewrite !Nat.mul_add_distr_r in *.
+      rewrite !Nat.add_assoc in *.
+      omega. (* Oh [omega], my dear [omega]! *)
+  Qed.
+
+
+  Lemma Iter_Terminates :
+    projT1 Iter ↓ (fun tin k => exists x y, tin[@Fin.F1] ≂ x /\ tin[@Fin.FS Fin.F1] ≂ y /\ Iter_steps x y <= k).
+  Proof.
+    unfold Iter. eapply While_TerminatesIn.
+    - eapply Iter_step_Computes.
+    - eapply Iter_step_terminates.
+    - intros tin k (x&y&HeX&HeY&Hk).
+      destruct y as [ | y' ] eqn:Ey.
+      + exists 6. repeat split.
+        * exists x, y. subst. auto.
+        * intros b () tout (HComp1&HComp2). specialize (HComp1 _ HeY) as (HComp11&HComp12). specialize (HComp2 _ _ HeX HeY).
+          cbn -[plus add] in *. cbv in HComp12. inv HComp12. auto.
+      + exists (6 + M1_runtime x). repeat split.
+        * exists x, y. subst. repeat split; auto.
+        * intros b () tout (HComp1&HComp2). specialize (HComp1 _ HeY) as (HComp11&HComp12). specialize (HComp2 _ _ HeX HeY).
+          cbn -[plus add] in *. cbv in HComp12. inv HComp12.
+          eexists. repeat split.
+          -- eauto.
+          -- rewrite <- Hk. omega.
+  Qed.
+  
+End Iter1.
+
+
+Lemma add_steps : forall m n, Iter_steps S (fun _ => 5) m n = 6 + 12 * n.
 Proof.
-  eapply RealiseIn_monotone.
-  {
-    unfold Add_step. repeat TM_Correct.
-    + eapply MatchNat_Sem.
-    + eapply Constr_S_Sem.
-  }
-  { cbn. omega. }
-  {
-    intros tin (yout, tout). split.
-    - intros n HEn. destruct H; hnf in H.
-      + destruct H as (tmid&(H1&H2)&([]&t)&H3&->&->); hnf in H1, H2, H3. simpl_not_in.
-        specialize (H1 n). spec_assert H1 as (n'&->&H1). { unfold reorder. now simpl_vector. } cbn in *. split; auto.
-        destruct H3 as (H3&H4); hnf in H3, H4. simpl_not_in. rewrite <- H2, H4 in *; clear H2 H4. auto.
-      + destruct H as (tmid&(H1&H2)&->&->); hnf in H1, H2. simpl_not_in. specialize (H1 n).
-        spec_assert H1 as (->&H1). { unfold reorder. now simpl_vector. } cbn. auto.
-    - intros n m HEn Hem. destruct H; hnf in H.
-      + destruct H as (tmid&(H1&H2)&([]&t)&H3&->&->); hnf in H1, H2, H3. simpl_not_in.
-        specialize (H1 n). spec_assert H1 as (n'&->&H1). { unfold reorder. now simpl_vector. } cbn in *. split; auto.
-        destruct H3 as (H3&H4); hnf in H3, H4. simpl_not_in. rewrite <- H2, H4 in *; clear H2 H4. auto.
-      + destruct H as (tmid&(H1&H2)&->&->); hnf in H1, H2. simpl_not_in. specialize (H1 n). spec_assert H1 as (->&H1).
-        { unfold reorder. now simpl_vector. } cbn in *. rewrite H2 in *; clear H2. split; auto.
-  }
-Qed.
-
-Lemma Add_step_Computes_ignoreParam :
-  Add_step ⊨c(12)
-           Computes_Rel (Fin.F1) (Fin.F1) _ _ pred ∩
-           Computes2_Rel (Fin.F1) (Fin.FS Fin.F1) (Fin.FS Fin.F1) _ _ _ add_step__f.
-Proof.
-  eapply RealiseIn_monotone.
-  - eapply Add_step_Computes.
+  intros m n. revert m. induction n as [ | n' IH]; intros; cbn -[plus mult] in *.
   - omega.
-  - apply subrel_and2. split.
-    + apply Computes_Rel_ignore_param.
-    + apply Computes2_Rel_ignore_param.
+  - rewrite IH. omega.
 Qed.
 
 
-Definition Add : { M : mTM _ 2 & states M -> unit } := WHILE Add_step.
+Definition Add := Iter Constr_S.
 
-Lemma add_tail_pred_step (x y : nat) :
-  tail_plus (Init.Nat.pred x) (add_step__f x y) = tail_plus x y.
-Proof. rewrite <- !plus_tail_plus. destruct x, y; cbn; omega. Qed.
-
-
-Lemma Add_Sem' :
-  Add ⊫ Computes2_Rel (Fin.F1) (Fin.FS Fin.F1) (Fin.FS Fin.F1) _ _ _ tail_plus.
+Lemma tail_add_iter (m n : nat) :
+  tail_plus m n = iter S m n.
 Proof.
-  eapply WRealise_monotone.
-  {
-    unfold Add. TM_Correct. eapply RealiseIn_WRealise. eapply Add_step_Computes.
-  }
-  {
-    hnf. intros tin ((), tout) H. destruct H as (tmid&H1&H2&H3).
-    revert tout H2 H3. induction H1 as [ tin | tin tmid tout H1 H2 IH]; intros; hnf in *; intros.
-    - specialize (H2 _ H) as (H2&H2'). specialize (H3 _ _ H H0) as (H3&H3'). cbn in *.
-      unfold add_step__p1, add_step__p2 in *. destruct x, y; cbn in *; inv H2'; inv H3'; auto.
-    - cbn in *. destruct H1 as (()&H11&H12).
-      hnf in H11, H12. specialize (H11 x H) as (H11&H11'). specialize (H12 x y H H4) as (H12&H12').
-      specialize (IH _ H0 H3). specialize (IH _ _ H11 H12). now rewrite add_tail_pred_step in IH.
-  }
+  revert m. induction n; intros; cbn in *.
+  omega. rewrite IHn. omega.
 Qed.
 
-Lemma Add_Sem :
-  Add ⊫ Computes2_Rel (Fin.F1) (Fin.FS Fin.F1) (Fin.FS Fin.F1) _ _ _ Nat.add.
+Lemma Add_WRealise' :
+  Add ⊫ Computes2_Rel (Fin.F1) (Fin.FS Fin.F1) (Fin.F1) _ _ _ tail_plus.
 Proof.
   eapply Computes2_Ext_WRealise.
-  - apply plus_tail_plus.
-  - apply Add_Sem'.
+  - refine tail_add_iter.
+  - unfold Add. apply Iter_Computes.
+    eapply WRealise_monotone. 
+    + eapply RealiseIn_WRealise. apply Constr_S_Sem.
+    + intros tin ((), tout) H. hnf in *. auto.
+Qed.
+
+Lemma Add_Terminates :
+  projT1 Add ↓ (fun tin k => exists x y, tin[@Fin.F1] ≂ x /\ tin[@Fin.FS Fin.F1] ≂ y /\ 6 + 12 * y <= k).
+Proof.
+  eapply TerminatesIn_monotone.
+  - unfold Add. apply Iter_Terminates.
+    + eapply RealiseIn_WRealise. apply Constr_S_Sem.
+    + eapply TerminatesIn_monotone. eapply RealiseIn_terminatesIn. apply Constr_S_Sem.
+      instantiate (1 := fun _ => 5). intros. hnf.
+      destruct H as (?&?&H). omega.
+  - intros tin k. intros (x&y&HeX&HeY&Hk). exists x, y. repeat split; auto. rewrite <- Hk.
+    pose proof add_steps x y as ->. omega.
 Qed.
 
 
-
-(* * Termination *)
-
-Fixpoint step_count (n : nat) : nat :=
-  match n with
-  | O => 12
-  | S n' => 13 + step_count n'
-  end.
-
-Lemma step_count_ge_12 (n : nat) :
-  12 <= step_count n.
-Proof. induction n; cbn; omega. Qed.
-
-
-Lemma step_count_pred_ge_13 (n : nat) :
-  13 + step_count (Init.Nat.pred n) <= step_count n.
-Proof.
-  destruct n; cbn.
-Abort.
-
-
+(*
 Section Test.
   Let t0 := midtape [inl START] (inr false) (map inr [] ++ [inl STOP]).
   Let t1 := midtape [inl START] (inr true) (map inr [false] ++ [inl STOP]).
@@ -285,43 +326,14 @@ Section Test.
   Let t3 := midtape [inl START] (inr true) (map inr [true; true; false] ++ [inl STOP]).
   Let t4 := midtape [inl START] (inr true) (map inr [true; true; true; false] ++ [inl STOP]).
 
+  Let step_count n := 6 + 12 * n.
+
   Compute execTM_p Add (step_count 0) [|t0; t0|].
-  Compute execTM_p Add (step_count 0) [|t0; t4|].
-  Compute execTM_p Add (step_count 1) [|t1; t3|].
-  Compute execTM_p Add (step_count 2) [|t2; t3|].
+  Compute execTM_p Add (step_count 4) [|t0; t4|].
+  Compute execTM_p Add (step_count 3) [|t1; t3|].
+  Compute execTM_p Add (step_count 3) [|t2; t3|].
   Compute execTM_p Add (step_count 3) [|t3; t3|].
-  Compute execTM_p Add (step_count 3) [|t3; t4|].
-  Compute execTM_p Add (step_count 4) [|t4; t0|].
+  Compute execTM_p Add (step_count 4) [|t3; t4|].
+  Compute execTM_p Add (step_count 0) [|t4; t0|].
 End Test.
-
-
-
-Lemma Add_terminatesIn :
-  projT1 Add ↓ (fun tin steps => exists x y : nat, tin[@Fin.F1] ≂ x /\ tin[@Fin.FS Fin.F1] ≂ y /\ step_count x <= steps).
-Proof.
-  eapply While_TerminatesIn.
-  {
-    eapply RealiseIn_WRealise. eapply Add_step_Computes.
-  }
-  {
-    eapply RealiseIn_terminatesIn. eapply Add_step_Computes.
-  }
-  {
-    intros tin i (m&n&HEncM&HEncN&Hi). exists 12. split.
-    - omega.
-    - intros [ | ] () tout (HComp1&HComp2).
-      + specialize (HComp1 _ HEncM) as (HComp1&HComp1'). specialize (HComp2 _ _ HEncM HEncN) as (HComp2&HComp2').
-        unfold add_step__p1, add_step__p2, add_step__f, is_not_zero in *.
-        destruct m as [ | m'].
-        {
-          (* m must have been [false], since [m] is [0]. *)
-          exfalso. congruence.
-        }
-        {
-          eexists. split.
-          - do 2 eexists. split. eauto. split. eauto. eauto.
-          - cbn -[plus]. cbn -[plus] in Hi. rewrite Hi. omega.
-        }
-      + rewrite <- Hi. eapply step_count_ge_12.
-  }
-Qed.
+*)
